ems/SimModSemHint.v
@@ -1006,33 +1006,6 @@ Section SIMMOD.
      induction mds; ss. f_equal. rewrite <- IHmds. ss.
    Qed.
 
-   Lemma fold_right_app_flat_map A B (f: A -> list B) l
-     :
-       flat_map f l
-       =
-       fold_right (@app _) [] (List.map f l).
-   Proof.
-     induction l; ss. f_equal. auto.
-   Qed.
-
-   Lemma map_flat_map A B C (f: A -> list B) (g: B -> C) (l: list A)
-     :
-       List.map g (flat_map f l)
-       =
-       flat_map (List.map g) (List.map f l).
-   Proof.
-     induction l; ss. rewrite List.map_app. f_equal; auto.
-   Qed.
-
-   Lemma flat_map_single A B (f: A -> B) (l: list A)
-     :
-       flat_map (fun a => [f a]) l
-       =
-       List.map f l.
-   Proof.
-     induction l; ss.
-   Qed.
-
    Theorem adequacy_hint `{ns: sk_gnames} mds_src mds_tgt
           (NAMESPACE:
              forall sk fn
